---
title: "my cool title"
date: 2023-05-19
---

(i) It intertwines

    (a) translation with modulation:
$$\mathcal{F} (f(\bullet + y))(\xi) = e(\langle y, \xi \rangle) \mathcal{F} f(\xi),$$

    (b) modulation with translation:
$$\mathcal{F} (e(-\langle \bullet, \eta \rangle) f(\bullet))(\xi) = \mathcal{F} f(\xi + \eta),$$

    (c) linear substitutions with linear substitutions: for
        $A \in \mathop{\mathrm{GL}}(V)$,
$$\mathcal{F} (f(A \bullet))(\xi) = \frac{1}{|\det A|} \mathcal{F} f(A^{-%
          {\mathpalette\@transpose{}}%
        } \xi),$$

    (d) dilation with dilation (take $A$ to be a scalar operator):
$$\mathcal{F} (f(\lambda \bullet))(\xi) = \frac{1}{\lambda^n} \mathcal{F} f(\lambda^{-1} \xi),$$

    (e) orthogonal transformations with their inverses: for
        $A \in \operatorname{O}(V)$,
$$\mathcal{F} (f(A \bullet))(\xi) = \mathcal{F} f(A^{-1} \xi),$$

    (f) convolution with pointwise multiplication:
$$\mathcal{F} (f \ast g)(\xi) = \mathcal{F} f(\xi) \mathcal{F} g(\xi),$$
        where $f \ast g(x) := \int_V f(x - y) g(y) \, d y$,

    (g) pointwise multiplication with convolution:
$$\mathcal{F} (f g)(\xi) = \mathcal{F} f(\xi) \ast \mathcal{F} g(\xi),$$

    (h) differentiation with multiplication by polynomials:
$$\label{eqn:35abf44e9d}
              \mathcal{F} (\partial^\alpha f)(\xi) = (2 \pi i)^{|\alpha|} \xi^\alpha \mathcal{F} f(\xi),$$

    (i) multiplication by polynomials with differentiation:
$$\label{eqn:35abf44e9f}
              \mathcal{F} (x^\alpha f)(\xi) = (-2 \pi i)^{-|\alpha|} \partial^\alpha \mathcal{F} f(\xi).$$

(ii) It is an isometry on $L^2(V)$, that is, for all $f,g \in L^2(V)$,
     we have the *Parseval formula*
     $$\int_V f(x) \overline{g(x)} \, d x = \int_V \mathcal{F} f(\xi) \overline{\mathcal{F} g(\xi)} \, d \xi.$$

(iii) It defines a *topological automorphism* of the Schwartz space
      $\mathcal{S}(V)$. This property asserts, in view of the Fourier
      inversion formula, that for any pair of multi-indices
      $\alpha,\beta \in \mathbb{Z}_{\geq 0}^n$, there exists $C \geq 0$
      and a finite family of pairs of multi-indices
      $\{ (\alpha_i, \beta_i) \}_{i=1}^N$ such that for all
      $f \in \mathcal{S}(V)$,
      $$\lVert \mathcal{F} f \rVert_{\alpha, \beta } \leq C \sum_{i=1}^N \lVert f \rVert_{\alpha_i, \beta_i}.$$
      For the sake of illustration, we record the proof of this fact. We
      observe first that, since $\left\lvert e(z) \right\rvert \leq 1$,
      $$\sup_{\xi \in \mathbb{R}^n} \left\lvert \mathcal{F} f(\xi) \right\rvert \leq \lVert f \rVert_{L^1}.$$
      By [\[eqn:35abf44e9d\]](#eqn:35abf44e9d){reference-type="eqref"
      reference="eqn:35abf44e9d"} and
      [\[eqn:35abf44e9f\]](#eqn:35abf44e9f){reference-type="eqref"
      reference="eqn:35abf44e9f"}, it follows that for all
      $\alpha, \beta \in \mathbb{Z}_{\geq 0}^n$,
      $$\sup_{\xi \in \mathbb{R}^n} \left\lvert \xi^\alpha \partial^\beta \mathcal{F} f(\xi) \right\rvert \leq
          (2 \pi)^{|\beta|-|\alpha|}  \lVert \partial^{\beta} x^\alpha  f \rVert_{L^1}.$$
      Using the product rule for derivatives, we may write
      $$\partial ^{\beta} x^\alpha f = \sum_{
            \substack{
              \alpha ' \leq \alpha  \\
              \beta ' \leq \beta 
            }
          }
          C_{\alpha,\beta,\alpha ', \beta '} x^{\alpha '} \partial^{\beta '} f$$
      for some constants $C_{\alpha,\beta,\alpha ', \beta '}$. On the
      other hand, for any function $\phi$ on $V$, we have
      $$\lVert \phi  \rVert_{L^1} \leq \frac{1}{\int_{x \in V } (1 + |x|)^{n+1} \, d x} \sup_{x \in V} (1 + |x|)^{n+1} \left\lvert \phi(x) \right\rvert.$$
      The required estimate follows upon taking the pairs
      $(\alpha_i,\beta_i)$ to consist of all
      $(\alpha ' + \gamma , \beta ')$ with $\alpha ' \leq \alpha$,
      $\beta ' \leq \beta$ and $\lvert \gamma  \rvert \leq n + 1$.

For $\phi \in \mathcal{S}(V)$ and
$(q, p, A) \in V \times V^* \times \mathop{\mathrm{GL}}(V)$, let us
introduce the temporary notation $$\label{eqn:35abf4d2f9}
  \phi_{q, p, A}(x) := \lvert \det A  \rvert^{- 1/2} e(\langle x, p \rangle) \phi(A^{-1} (x - q)).$$

::: {#exercise:35ac01c3ef .exercise}
**Exercise 1**. Check the following.

(i) The functions $\phi$ and $\phi_{q,p,A}$ have the same $L^2$-norms.

(ii) We have $$\label{eqn:35ac01c434}
           \mathcal{F} \phi_{q, p, A} = e (\langle q, p \rangle) (\mathcal{F} \phi )_{p, -q, A^{-1}}.$$

(iii) For $\eta, y\in V \times V^*$,
      $$e (\langle \bullet , \eta \rangle ) \phi_{q,p,A} (\bullet - y)
            =
            \phi_{q + y, p + \eta, A},$$

(iv) For $B \in  \mathop{\mathrm{GL}}(V)$,
     $$\lvert \det B \rvert^{- 1/2} \phi_{q, p, A} (B^{-1} \bullet )
           = \phi_{B q, B^{-T} p, B A}.$$

(v) For a symmetric operator $B \in \mathop{\mathrm{End}}(V)$ and
    $f \in C^\infty(V)$, define
    $$\omega_B f (x) := e (\langle x, \tfrac{1}{2} B x \rangle) f (x).$$
    Then $$\omega_B \phi_{p, q, A} =
          e (- \langle q, \tfrac{1}{2} B q \rangle)
          \phi '_{q, p + B q, A},$$ where
    $$\phi ' (x) := e (\langle x, \tfrac{1}{2} A^T B A x \rangle) \phi (x).$$
:::

::: definition
**Definition 1**. Let $S$ be a subset of $\mathcal{S}(V)$, and let
$(q,p,A)$ be as above. We say that $f$ is $S$*-localized at* $(q, p, A)$
if there exists $\phi \in S$ so that $f = \phi_{q,p,A}$.
:::

By definition, a subset $S$ of the topological vector space
$\mathcal{S} (V)$ is *bounded* if for every pair of multi-indices
$\alpha,\beta \in \mathbb{Z}_{\geq 0}^n$, there exists $C \geq 0$ such
that for all $f \in S$, we have $\lVert f \rVert_{\alpha,\beta} \leq C$.
A subset $S$ of $\mathcal{S}(V)$ is *saturated* if $c f \in S$ whenever
$f \in S$ and $\lvert c \rvert \leq 1$. The topological automorphism
property of the Fourier transform may be restated as follows: the image
of each bounded (equivalently, each saturated and bounded) subset of
$\mathcal{S}(V)$ under the Fourier transform is bounded. By combining
this property with the intertwining property
[\[eqn:35ac01c434\]](#eqn:35ac01c434){reference-type="eqref"
reference="eqn:35ac01c434"} noted in Exercise
[1](#exercise:35ac01c3ef){reference-type="ref"
reference="exercise:35ac01c3ef"}, we obtain some understanding of how
the Fourier transform affects asymptotics.

